theories/logrel/ftlr_retrieve.v
@@ -1,0 +1,321 @@
+From iris.proofmode Require Import tactics.
+From machine_program_logic.program_logic Require Import weakestpre.
+From HypVeri.lang Require Import lang trans_extra.
+From HypVeri.algebra Require Import base pagetable mem trans.
+From HypVeri.rules Require Import mem_retrieve.
+From HypVeri.logrel Require Import logrel logrel_extra.
+From HypVeri Require Import proofmode stdpp_extra.
+Import uPred.
+
+Section ftlr_retrieve.
+  Context `{hypconst:HypervisorConstants}.
+  Context `{hypparams:!HypervisorParameters}.
+  Context `{vmG: !gen_VMG Σ}.
+
+Lemma ftlr_retrieve {i trans' mem_acc_tx ai regs ps_acc p_tx p_rx ps_na instr trans rx_state r0}:
+  base_extra.is_total_gmap regs ->
+  {[p_tx; p_rx]} ⊆ ps_acc ->
+  i ≠ V0 ->
+  ps_na ## ps_acc ∪ pages_in_trans (trans_memory_in_trans i trans) ->
+  p_rx ∉ ps_acc ∖ {[p_rx; p_tx]} ∪ pages_in_trans (trans_memory_in_trans i trans) ->
+  p_tx ∉ ps_acc ∖ {[p_rx; p_tx]} ∪ pages_in_trans (trans_memory_in_trans i trans) ->
+  regs !! PC = Some ai ->
+  tpa ai ∈ ps_acc ->
+  tpa ai ≠ p_tx ->
+  dom (gset Addr) mem_acc_tx = set_of_addr (ps_acc ∖ {[p_tx]}) ->
+  tpa ai ∈ ps_acc ∖ {[p_tx]} ->
+  mem_acc_tx !! ai = Some instr ->
+  decode_instruction instr = Some Hvc ->
+  regs !! R0 = Some r0 ->
+  decode_hvc_func r0 = Some Retrieve ->
+  p_tx ≠ p_rx ->
+  ⊢
+  ▷ (∀ (a : gmap reg_name Addr) (a0 : gset PID) (a1 : gmap Addr transaction) (a2 : option (Addr * VMID)),
+          ⌜base_extra.is_total_gmap a⌝
+            → ⌜{[p_tx; p_rx]} ⊆ a0⌝
+              → ⌜ps_na ## a0 ∪ pages_in_trans (trans_memory_in_trans i a1)⌝
+                → ⌜p_rx ∉ a0 ∖ {[p_rx; p_tx]} ∪ pages_in_trans (trans_memory_in_trans i a1)⌝
+                  → ⌜p_tx ∉ a0 ∖ {[p_rx; p_tx]} ∪ pages_in_trans (trans_memory_in_trans i a1)⌝
+                    → ([∗ map] r↦w ∈ a, r @@ i ->r w) -∗
+                      TX@i:=p_tx -∗
+                      p_tx -@O> - ∗ p_tx -@E> true -∗
+                      i -@{1 / 2}A> a0 -∗
+                      i -@{1 / 2}A> a0 -∗
+                      LB@ i := [ps_na] -∗
+                      transaction_hpool_global_transferred a1 -∗
+                      transaction_pagetable_entries_transferred i a1 -∗
+                      retrieval_entries i a1 -∗
+                      R0 @@ V0 ->r encode_hvc_func Run -∗
+                      R1 @@ V0 ->r encode_vmid i -∗
+                      RX_state@i:= a2 -∗
+                      mailbox.rx_page i p_rx -∗
+                      ▷ VMProp V0 (vmprop_zero i p_rx) (1 / 2) -∗
+                      VMProp i (vmprop_unknown i p_tx p_rx trans') 1 -∗
+                      transaction_pagetable_entries_owned i a1 -∗
+                      pagetable_entries_excl_owned i (a0 ∖ {[p_rx; p_tx]} ∖ pages_in_trans a1) -∗
+                      (∃ mem : lang.mem, memory_pages (a0 ∪ pages_in_trans (trans_memory_in_trans i a1)) mem) -∗
+                      WP ExecI @ i {{ _, True }}) -∗
+   ([∗ map] r↦w ∈ regs, r @@ i ->r w) -∗
+   TX@i:=p_tx -∗
+   p_tx -@O> - ∗ p_tx -@E> true -∗
+   i -@{1 / 2}A> ps_acc -∗
+   i -@{1 / 2}A> ps_acc -∗
+   LB@ i := [ps_na] -∗
+   transaction_hpool_global_transferred trans -∗
+   transaction_pagetable_entries_transferred i trans -∗
+   retrieval_entries i trans -∗
+   R0 @@ V0 ->r encode_hvc_func Run -∗
+   R1 @@ V0 ->r encode_vmid i -∗
+   RX_state@i:= rx_state -∗
+   mailbox.rx_page i p_rx -∗
+   ▷ VMProp V0 (vmprop_zero i p_rx) (1 / 2) -∗
+   VMProp i (vmprop_unknown i p_tx p_rx trans') 1 -∗
+   transaction_pagetable_entries_owned i trans -∗
+   pagetable_entries_excl_owned i (ps_acc ∖ {[p_rx; p_tx]} ∖ pages_in_trans trans) -∗
+   (∃ mem1 : mem, memory_pages ((ps_acc ∪ (pages_in_trans (trans_memory_in_trans i trans))) ∖ ps_acc) mem1) -∗
+   ([∗ map] k↦v ∈ mem_acc_tx, k ->a v) -∗
+   (∃ mem2 : mem, memory_page p_tx mem2) -∗
+   SSWP ExecI @ i {{ bm, (if bm.1 then VMProp_holds i (1 / 2) else True) -∗ WP bm.2 @ i {{ _, True }} }}.
+  Proof.
+    iIntros (Htotal_regs Hsubset_mb Hneq_0 Hdisj_na Hnin_rx Hnin_tx Hlookup_PC Hin_ps_acc Hneq_ptx Hdom_mem_acc_tx Hin_ps_acc_tx
+                         Hlookup_mem_ai Heqn  Hlookup_reg_R0 Hdecode_hvc).
+    iIntros (Hneq_mb) "IH regs tx pgt_tx pgt_acc pgt_acc' LB trans_hpool_global tran_pgt_transferred retri R0z R1z rx_state rx prop0
+             propi tran_pgt_owned pgt_owned mem_rest mem_acc_tx mem_tx".
+    set ps_mem_in_trans := (pages_in_trans (trans_memory_in_trans i trans)).
+    pose proof (Htotal_regs R1) as[r1 Hlookup_reg_R1].
+    pose proof (Htotal_regs R2) as[r2 Hlookup_reg_R2].
+    iDestruct (reg_big_sepM_split_upd4 i Hlookup_PC Hlookup_reg_R0 Hlookup_reg_R1 Hlookup_reg_R2 with "[$regs]")
+      as "(PC & R0 & R1 & R2 & Hacc_regs)";eauto.
+
+    iDestruct "rx" as "[rx pgt_rx]".
+
+    iDestruct (access_split with "[$pgt_acc $pgt_acc']") as "pgt_acc".
+
+    iDestruct "trans_hpool_global" as (hpool) "(%Heq_hsall & fresh_handles & %Htrans_ps_disj & trans)".
+    destruct (decide (r1 ∈ hs_all)) as [Hin_hs_all |Hnotin_hs_all].
+    2: { (* apply [hvc_mem_retrieve_invalid_handle] *)
+      admit.
+    }
+    destruct (decide (r1 ∈ hpool)) as [Hin_hpool | Hnotin_hpool].
+    { (* apply [hvc_mem_retrieve_fresh_handle] *)
+      admit.
+    }
+    assert(r1 ∈ dom (gset _ ) trans) as Hin_trans_dom.
+    {
+      rewrite -Heq_hsall in Hin_hs_all.
+      rewrite elem_of_union in Hin_hs_all.
+      destruct Hin_hs_all;first contradiction.
+      done.
+    }
+    apply elem_of_dom in Hin_trans_dom as [tran Hlookup_tran].
+    iDestruct (big_sepM_delete _ trans _  _ Hlookup_tran with "trans") as "(tran & trans)".
+
+    destruct(decide (tran.1.1.1.2 = i)) as [Heq_tran | Hneq_tran].
+    2: { (*apply [hvc_mem_retrieve_invalid_trans]*)
+      admit.
+    }
+
+    iDestruct ("retri") as "[retri retri']".
+    iDestruct (big_sepFM_lookup_Some Hlookup_tran with "retri") as "[re retri]".
+    simpl;left;done.
+
+    destruct (tran.2) eqn:Heq_retri.
+    { (* apply [hvc_mem_retrieve_retrieved] *)
+      admit.
+    }
+
+    iDestruct (big_sepFM_lookup_Some Hlookup_tran with "retri'") as "[re' retri']".
+    simpl;left;split;done.
+    rewrite Heq_retri.
+    iDestruct (retri_split with "[$re $re']") as "re".
+
+    destruct (rx_state)  eqn: Heq_rxstate.
+    { (* apply [hvc_mem_retrieve_rx_full] *)
+      admit.
+    }
+
+    assert (tran.1.1.2 ⊆ ps_mem_in_trans) as Hsubseteq_tran.
+    {
+      rewrite elem_of_subseteq.
+      intros p Hin_p.
+      rewrite /ps_mem_in_trans.
+      rewrite elem_of_pages_in_trans.
+      exists r1, tran.
+      split;last auto.
+      rewrite map_filter_lookup_Some;split;first done.
+      simpl. right;done.
+    }
+
+    assert (p_rx ∈ ps_acc ∖ {[p_tx]}) as Hin_ps_acc_tx'. set_solver + Hsubset_mb Hneq_mb.
+    iDestruct (memory_pages_split_singleton p_rx _ Hin_ps_acc_tx') as "[Hsplit _]".
+    iDestruct ("Hsplit" with "[mem_acc_tx]") as (mem_acc_tx_rx mem_rx) "[[%Hdom_mem_acc_tx_rx mem_acc_tx_rx] [mem_rx %Heq_mem_acc_tx_rx]]".
+    {
+      rewrite /memory_pages.
+      iSplitL "".
+      iPureIntro.
+      apply Hdom_mem_acc_tx.
+      iFrame.
+    }
+    iClear "Hsplit".
+    rewrite -Heq_mem_acc_tx_rx in Hlookup_mem_ai.
+    iAssert (⌜dom (gset _) mem_rx = set_of_addr {[p_rx]}⌝)%I as "%Hdom_mem_rx".
+    {
+      rewrite set_of_addr_singleton.
+      iDestruct "mem_rx" as "[$ _]".
+    }
+    rewrite lookup_union_Some in Hlookup_mem_ai.
+    2:{ apply map_disjoint_dom. rewrite Hdom_mem_acc_tx_rx Hdom_mem_rx.
+        apply set_of_addr_disj.
+        set_solver +.
+    }
+
+    destruct (tran.1.2) eqn:Heq_tran_tt.
+    { (*apply [hvc_mem_retrieve_donate]*)
+      iDestruct (big_sepFM_lookup_Some Hlookup_tran with "tran_pgt_transferred") as "[[tran' [own_tran excl_tran]] tran_pgt_transferred]".
+      simpl. split;first done. left;done.
+      iDestruct (trans_split with "[$tran $tran']") as "tran".
+
+      destruct Hlookup_mem_ai as [Hlookup_mem_ai|Hlookup_mem_ai].
+      {
+        iDestruct (mem_big_sepM_split mem_acc_tx_rx Hlookup_mem_ai with "mem_acc_tx_rx") as "[mem_instr Hacc_mem_acc_tx_rx]".
+        assert(tran.1 = (tran.1.1.1.1.1, tran.1.1.1.1.2, i, tran.1.1.2, Donation)) as ?.
+        {
+          rewrite -Heq_tran_tt.
+          rewrite -Heq_tran.
+          repeat destruct tran as [tran ?]. simpl. done.
+        }
+        rewrite H; clear H.
+
+        iApply (hvc_mem_retrieve_donate ai r1 with "[$PC $mem_instr $R0 $R1 $own_tran $pgt_acc $re $tran $rx $rx_state $mem_rx $fresh_handles]").
+        set_solver + Hin_ps_acc_tx.
+        done.
+        done.
+        iNext.
+        simpl.
+        iIntros "(PC & mem_instr & R0 & R1 & own_tran & pgt_acc & rx & (%wl & %des & rx_state & _ & _ & mem_rx) & fresh_handles) _".
+
+        iDestruct ("Hacc_regs" $! (ai ^+ 1)%f with "[$ PC $ R0 $ R1 $ R2]") as (regs') "[%Htotal_regs' regs]".
+        iDestruct ("Hacc_mem_acc_tx_rx" with "[$mem_instr]") as "mem_acc_tx_rx".
+        iDestruct (access_split with "pgt_acc") as "[pgt_acc pgt_acc']".
+
+        assert (pages_in_trans (trans_memory_in_trans i (delete r1 trans)) = ps_mem_in_trans ∖ tran.1.1.2) as Hrewrite.
+        {
+          rewrite /trans_memory_in_trans.
+          rewrite map_filter_delete.
+          apply pages_in_trans_delete.
+          rewrite map_filter_lookup_Some.
+          split;first done.
+          simpl. right. done.
+          apply (trans_ps_disj_subseteq trans).
+          done.
+          apply map_filter_subseteq.
+        }
+
+        iApply ("IH" $! _ _ (delete r1 trans) _ Htotal_regs' _ _ _ _ with "regs tx pgt_tx pgt_acc pgt_acc' LB [fresh_handles trans]
+                            [tran_pgt_transferred] [retri retri'] R0z R1z rx_state [$rx $pgt_rx] prop0 propi [tran_pgt_owned]
+                            [own_tran excl_tran pgt_owned] [mem_rest mem_acc_tx_rx mem_rx mem_tx]").
+        {
+          iExists (hpool ∪ {[r1]}).
+          iFrame "fresh_handles trans".
+          iPureIntro.
+          assert (r1 ∈ dom (gset _) trans).
+          {
+            rewrite elem_of_dom.
+            exists tran;done.
+          }
+          rewrite union_comm_L in Heq_hsall.
+          rewrite -Heq_hsall.
+          rewrite union_comm_L.
+          rewrite (union_comm_L hpool).
+          rewrite union_assoc_L.
+          f_equal.
+          rewrite dom_delete_L.
+          rewrite difference_union_L.
+          split.
+          set_solver + H.
+          apply (trans_ps_disj_subseteq trans).
+          done.
+          apply map_subseteq_delete.
+        }
+        {
+          rewrite /transaction_pagetable_entries_transferred.
+          done.
+        }
+        {
+          rewrite /retrieval_entries.
+          iFrame "retri retri'".
+        }
+        {
+          rewrite /transaction_pagetable_entries_owned.
+          rewrite (big_sepFM_delete_False Hlookup_tran).
+          iFrame "tran_pgt_owned".
+          simpl.
+          intros [_ ?].
+          contradiction.
+        }
+        {
+          assert (pages_in_trans (delete r1 trans) = pages_in_trans trans ∖ tran.1.1.2) as ->.
+          {
+            apply pages_in_trans_delete;auto.
+          }
+          rewrite (difference_union_distr_l_L tran.1.1.2).
+          assert (tran.1.1.2 ∖ {[p_rx;p_tx]} = tran.1.1.2) as ->.
+          set_solver + Hnin_rx Hnin_tx Hsubseteq_tran.
+          rewrite (difference_union_distr_l_L tran.1.1.2).
+          assert (tran.1.1.2 ∖ (pages_in_trans trans ∖ tran.1.1.2) = tran.1.1.2) as ->.
+          set_solver + Hsubseteq_tran.
+          assert (ps_mem_in_trans ⊆ pages_in_trans trans) as Hsub.
+          apply pages_in_trans_subseteq.
+          apply map_filter_subseteq.
+          assert (tran.1.1.2 ∪ ps_acc ∖ {[p_rx; p_tx]} ∖ (pages_in_trans trans ∖ tran.1.1.2) = tran.1.1.2 ∪ ps_acc ∖ {[p_rx; p_tx]} ∖ pages_in_trans trans) as ->.
+          set A := (ps_acc ∖ {[p_rx; p_tx]}).
+          set G := (tran.1.1.2 ∪ A ∖ (pages_in_trans trans ∖ tran.1.1.2)).
+
+          rewrite (union_difference_L tran.1.1.2 (pages_in_trans trans) ).
+          2: {
+            set_solver + Hsub Hsubseteq_tran.
+          }
+          rewrite difference_union_distr_r_L.
+          rewrite union_intersection_l_L.
+          rewrite (union_comm_L tran.1.1.2).
+          rewrite difference_union_L.
+          rewrite intersection_comm_L.
+          symmetry.
+          rewrite /G.
+          rewrite subseteq_intersection_1_L. done.
+          set_solver +.
+          iDestruct "pgt_owned" as "[own_owned excl_owned]".
+          iSplitL "own_owned own_tran".
+          iApply (big_sepS_union with "[$own_tran $own_owned]").
+          set_solver + Hsubseteq_tran Hsub.
+          iApply (big_sepS_union with "[$excl_tran $excl_owned]").
+          set_solver + Hsubseteq_tran Hsub.
+        }
+        {
+          rewrite Hrewrite.
+          rewrite (union_comm_L tran.1.1.2).
+          rewrite -(union_assoc_L ps_acc tran.1.1.2).
+          rewrite -(union_difference_L tran.1.1.2);last set_solver + Hsubseteq_tran.
+          iApply (memory_pages_split_diff' _ ps_acc).
+          set_solver +.
+          iSplitL "mem_rest"; first done.
+          iDestruct (memory_pages_split_singleton' p_rx with "[mem_acc_tx_rx mem_rx]") as "mem_acc_tx". set_solver + Hsubset_mb.
+          iSplitL "mem_acc_tx_rx".
+          iExists mem_acc_tx_rx; by iFrame "mem_acc_tx_rx".
+          iExists (list_to_map (zip (finz.seq p_rx (length des)) des) ∪ mem_rx); by iFrame "mem_rx".
+          iApply (memory_pages_split_singleton' p_tx with "[$mem_acc_tx $mem_tx]"). set_solver + Hsubset_mb.
+        }
+      }
+      { (* apply [hvc_mem_retrieve_donate_rx]*)
+        admit.
+      }
+    }
+    { (* apply [hvc_mem_retrieve_share]*)
+      admit.
+    }
+    { (*apply [hvc_mem_retrieve_lend]*)
+      admit.
+    }
+  Admitted.
+
+End ftlr_retrieve.
